src/fs/nfs.s.dfy
@@ -39,6 +39,124 @@ module Nfs {
     ino in data && data[ino].DirFile?
   }
 
+  datatype RenameArgs = RenameArgs(
+    src: FsKinds.Ino, src_name: seq<byte>,
+    dst: FsKinds.Ino, dst_name: seq<byte>)
+  {
+    predicate Valid()
+    {
+      DirEntries.is_pathc(src_name) && DirEntries.is_pathc(dst_name)
+    }
+
+    predicate same_dir()
+    {
+      src == dst
+    }
+
+    predicate trivial()
+    {
+      same_dir() && src_name == dst_name
+    }
+  }
+
+  predicate rename_overwrite_ok(args: RenameArgs, data: Fs)
+  {
+    && args.Valid()
+    && is_dir_fs(args.src, data)
+    && is_dir_fs(args.dst, data)
+    && args.src_name in data[args.src].dir
+  }
+
+  function rename_overwrite_spec(args: RenameArgs, data: Fs): Fs
+    requires rename_overwrite_ok(args, data)
+  {
+    var srcd := data[args.src];
+    var srcf := srcd.dir[args.src_name];
+    var srcd' := srcd.delete(args.src_name);
+    var data1: Fs := data[args.src := srcd'];
+    var dstd := data1[args.dst];
+    var dstd' := DirFile(dstd.dir[args.dst_name := srcf], dstd.attrs);
+    data1[args.dst := dstd']
+  }
+
+  // simpler re-statement of rename_overwrite_spec_ok when src and destination coincide,
+  // mainly to demonstrate that rename_overwrite_spec is sensible
+  function rename_overwrite_spec_same_dir(args: RenameArgs, data: Fs): Fs
+    requires args.src == args.dst
+    requires rename_overwrite_ok(args, data)
+  {
+    var d0 := data[args.src];
+    var srcf := d0.dir[args.src_name];
+    var d := map_delete(d0.dir, args.src_name);
+    var d := d[args.dst_name := srcf];
+    data[args.src := DirFile(d, d0.attrs)]
+  }
+
+  lemma rename_overwrite_spec_same_dir_ok(args: RenameArgs, data: Fs)
+    requires rename_overwrite_ok(args, data)
+    requires args.src == args.dst
+    ensures rename_overwrite_spec_same_dir(args, data) == rename_overwrite_spec(args, data)
+  {
+  }
+
+  // after the core rename operation, will overwriting the destination file be
+  // valid?
+  //
+  // note that data is before the entire operation; after the initial rename
+  // the destination is lost so there isn't enough information to decide this
+  predicate rename_cleanup_ok(args: RenameArgs, data: Fs)
+    requires is_dir_fs(args.src, data) && is_dir_fs(args.dst, data)
+    requires args.src_name in data[args.src].dir
+  {
+    // we evaluate some of the following after removing the src, which might
+    // make a no-op rename valid or make it valid to rename a directory on top
+    // of its parent
+    var data1: Fs := data[args.src := data[args.src].delete(args.src_name)];
+    // there are three ways for the overwrite to be valid:
+    var dst1 := data1[args.dst];
+    // (1) the destination didn't exist so no overwriting took place
+    || (args.dst_name !in dst1.dir)
+    || var src := data[args.src];
+      var dst := data[args.dst];
+      && var src_ino := src.dir[args.src_name];
+        var dst_ino := dst.dir[args.dst_name];
+        // (2) source and destination are both files
+        || (&& is_file_fs(src_ino, data)
+          && is_file_fs(dst_ino, data))
+        // (3) source and destinations are both directories, and the
+        // destination is empty
+        || (&& is_dir_fs(src_ino, data)
+          && is_dir_fs(dst_ino, data)
+          && data1[dst_ino].dir == map[])
+  }
+
+  // rename with cleanup of any overwritten files
+  //
+  // note this is the entire rename spec, since the original data is needed to
+  // express the right cleanup
+  function rename_spec(args: RenameArgs, data: Fs): Fs
+    requires is_dir_fs(args.src, data) && is_dir_fs(args.dst, data)
+    requires rename_overwrite_ok(args, data)
+  {
+    // get the old destination file
+    var dst := data[args.dst];
+    var data: Fs := rename_overwrite_spec(args, data);
+    // no cleanup needed if destination didn't exist or src and dst refer to
+    // the same file
+    if args.dst_name !in dst.dir || args.trivial()
+    then data
+    else
+      var dst_ino := dst.dir[args.dst_name];
+      map_delete(data, dst_ino)
+  }
+
+  predicate rename_ok(args: RenameArgs, data: Fs)
+  {
+    && rename_overwrite_ok(args, data)
+    && rename_cleanup_ok(args, data)
+  }
+
+
   datatype Error =
     | Noent
     | Exist
